\begin{proofbox}\nospacing
    \begin{proof}[TVD FVM REA Scheme]\label{proof:lemma:tvd_fvm_rea_scheme}
        From\cref{eq:linear_reconstruction_approximation} we know:
        \begin{align*}
          u_{\idxj^{+}}^{n}&=u_{\idxj}^{n}+\frac{\sigmac_{\idxj}^{n}}{2}\Delta x=u_{\idxj}^{n}+\frac{\deltac_{\idxj}^{n}}{2}\\[-1\jot]
          u_{\idxj^{-}}^{n}&=u_{\idxj}^{n}-\frac{\sigmac_{\idxj}^{n}}{2}\Delta x=u_{\idxj}^{n}-\frac{\deltac_{\idxj}^{n}}{2}
        \end{align*}
        \begin{align*}
          T_{1}=&\frac{u_{\idxj+1}^{n}-\frac{\deltac_{\idxj-1}^{n}}{2}-u_{\idxj}^{n}+\frac{\deltac_{\idxj}^{n}}{2}}{u_{\idxj+1}^{n}-u_{\idxj}^{n}}\\[-1\jot]
          =&1-\frac{1}{2}\left[\frac{\deltac_{\idxj+1}^{n}-\deltac_{\idxj}^{n}}{u_{\idxj+1}^{n}-u_{\idxj}^{n}}\right]\\[-1\jot]
          T_{2}=&1+\frac{1}{2}\left[\frac{\deltac_{\idxj+1}^{n}-\deltac_{\idxj}^{n}}{u_{\idxj+1}^{n}-u_{\idxj}^{n}}\right]
        \end{align*}
        \begin{align*}
          \implies T_{1}+T_{2}\equiv2
        \end{align*}
        and the rest follows from the condition that $T_{1},T_{2}\geq0$
    \end{proof}
\end{proofbox}
\begin{proofbox}\nospacing
    \begin{proof}[TVD Minmod Limiter\cref{cor:minmod_is_tvd},\cref{lemma:tvd_fvm_rea_scheme}]\label{proof:tvd_minmod_limiter}
        \scalematho{
        \begin{align*}
          \frac{\deltac_{\idxj}^{n}}{u_{\idxj+1}-u_{\idxj}^{n}}=&\frac{\Delta x\sigmac_{\idxj}^{n}}{u_{\idxj+1}-u_{\idxj}^{n}}=
         \frac{\text{minmod} \left(u_{\idxj+1}^{n}-u_{\idxj}^{n},u_{\idxj}^{n}-u_{\idxj-1}^{n}\right)}{u_{\idxj+1}-u_{\idxj}^{n}}
        \end{align*}}
      \begin{align*}
        \text{sign}(u_{\idxj+1}^{n}-u_{\idxj}^{n})\neq\text{sign}(u_{\idxj}^{n}-u_{\idxj-1}^{n})&&\implies\sigmac_{\idxj}^{n}=0
      \end{align*}
      \begin{align*}
        \text{sign}(u_{\idxj+1}^{n}-u_{\idxj}^{n})=\text{sign}(u_{\idxj}^{n}-u_{\idxj-1}^{n})=\pm1
      \end{align*}
      \begin{align*}
        \implies\quad\frac{\deltac_{\idxj}^{n}}{u_{\idxj+1}-u_{\idxj}^{n}}=&\text{minmod}\left(\frac{{u_{\idxj+1}-u_{\idxj}^{n}}}{u_{\idxj+1}-u_{\idxj}^{n}},\frac{{u_{\idxj+1}-u_{\idxj}^{n}}}{u_{\idxj+1}-u_{\idxj}^{n}}\right)\\[-1\jot]
        =&\text{minmod}\Big(1,\underbrace{\frac{{u_{\idxj+1}-u_{\idxj}^{n}}}{u_{\idxj+1}-u_{\idxj}^{n}}}_{\geq0}\Big)\leq 1
      \end{align*}
      \begin{align*}
        \implies\quad 0\leq\frac{\deltac_{\idxj}^{n}}{u_{\idxj+1}-u_{\idxj}^{n}}\leq 1&&0\leq\frac{\deltac_{\idxj+1}^{n}}{u_{\idxj+1}-u_{\idxj}^{n}}\leq 1
      \end{align*}
      \begin{align}
        \implies&-1\leq\frac{\deltac_{\idxj+1}^{n}-\deltac_{\idxj}^{n}}{u_{\idxj+1}-u_{\idxj}^{n}}\leq 1
      \end{align}
    \end{proof}
\end{proofbox}

%%% Local Variables:
%%% mode: latex
%%% TeX-command-extra-options: "-shell-escape"
%%% TeX-master: "../../../../formulary"
%%% End:
