\begin{proofbox}\nospacing
    \begin{proof}[Decoupled hyperbolic lin. Cons. Law.\cref{proposition:decoupled_hyperbolic_lin_cons_law}]\label{proof:proposition:decoupled_hyperbolic_lin_cons_law}
        \begin{align*}
          \Uvec_{t}+\Avec\Uvec_{x}=0&& \\[-1\jot]
          \Uvec_{t}+\vec{R}\Lambdac\vec{R}^{-1}\Uvec_{x}=0&&\Cref{eq:eigendecomposition}\\[-1\jot]
          (\vec{R}^{-1}\Uvec)_{t}+\vec{R}^{-1}\vec{R}\Lambdac(\vec{R}^{-1}\Uvec)_{x}=0&&\text{Multiplying by $\vec{R}^{-1}$}\\[-1\jot]
          \Wvec_{t}+\Lambdac\Wvec_{x}=0&&\Wvec:=\vec{R}^{-1}\Uvec
        \end{align*}
    \end{proof}
\end{proofbox}
\begin{proofbox}\nospacing
    \begin{proof}[Jump Decomposition\cref{cor:jump_decomposition}]\label{proof:cor:jump_decomposition}
        \begin{align*}
          \Uvec_{R}-\Uvec_{L}=\vec{R}(\Wvec_{R}-\Wvec_{L})&=\sum_{\idxp=1}^{\idxm}\left(W_{R}^{\idxp}-W_{L}^{\idxp}\right)r_{\idxp}\nonumber\\[-1\jot]
          &:=\sum_{\idxp=1}^{\idxm}\alphac^{\idxp}r_{\idxp}
        \end{align*}
    \end{proof}
\end{proofbox}

%%% Local Variables:
%%% mode: latex
%%% TeX-command-extra-options: "-shell-escape"
%%% TeX-master: "../../../formulary"
%%% End:
